format-version: 1.2
date: 10:01:2013 13:21
saved-by: djs93
auto-generated-by: OBO-Edit 2.2
default-namespace: FlyBase development CV
remark: Drosophila temporal ontology.
ontology: FBdv

[Term]
id: BFO:0000003
name: occurrent
def: "An entity that has temporal parts and that happens, unfolds or develops through time. Sometimes also called perdurants." [BFOC:ANON]

[Term]
id: FBdv:00005259
name: developmental stage
alt_id: FBdv:00007010
def: "A temporal subdivision of a developmental process." [FBC:DOS]
is_a: FBdv:00007008 ! occurrent
created_by: djs93
creation_date: 2009-10-01T05:56:56Z

[Term]
id: FBdv:00005289
name: embryonic stage
def: "The stage of the Drosophila life-cycle from fertilisation to hatching." [FBC:DOS]
comment: Temporal ordering number - 20.
is_a: FBdv:00007012 ! life stage

[Term]
id: FBdv:00005336
name: larval stage
def: "The stage of the Drosophila life-cycle from hatching to the beginning of puparium formation." [FBC:DOS]
comment: Temporal ordering number - 400.
is_a: FBdv:00007012 ! life stage
relationship: starts_at_end_of FBdv:00005289 ! embryonic stage

[Term]
id: FBdv:00005337
name: first instar larval stage
def: "The first larval instar begins at hatching and ends at the first larval molt. Anterior spiracles are not yet present; posterior spiracles have two openings each. Salivary glands are very small and all cells are uniform in size. Mouth hooks typically have one tooth. Duration at 25 degrees C: approximately 25 hours (24-49 hours after egg laying; 0-25 hours after hatching)." [FlyBase:FBrf0007733]
comment: Temporal ordering number - 410.
synonym: "first instar larva" EXACT []
synonym: "L1" EXACT []
is_a: FBdv:00007012 ! life stage
relationship: part_of FBdv:00005336 ! larval stage
relationship: starts_at_end_of FBdv:00005289 ! embryonic stage

[Term]
id: FBdv:00005338
name: second instar larval stage
def: "The second larval instar begins at the first larval molt and ends at the second larval molt. Larvae are actively feeding and crawling in the food. Distinct anterior spiracles are present as enlargements at the end of the tracheal trunk, but not open to the outside; posterior spiracles have three openings each, and four groups of small unbranched hairs. The salivary glands extend to the first abdominal segment, and have cells that are uniform in size. Mouth hooks typically have two or three teeth. Duration at 25 degrees C: approximately 23 hours (49-72 hours after egg laying; 25-48 hours after hatching)." [FlyBase:FBrf0007733]
comment: Temporal ordering number - 420.
synonym: "L2" EXACT []
synonym: "second instar larva" EXACT []
is_a: FBdv:00007012 ! life stage
relationship: part_of FBdv:00005336 ! larval stage
relationship: starts_at_end_of FBdv:00005337 ! first instar larval stage

[Term]
id: FBdv:00005339
name: third instar larval stage
def: "The third larval instar begins at the second larval molt and ends at puparium formation. Anterior spiracles are open to the outside; posterior spiracles have three openings each, and four groups of large branched hairs. The salivary glands extend to the second abdominal segment, with cells larger in the posterior than in the anterior of the gland. Mouth hooks typically have 9-12 teeth. About 24 hours before pupariation (at 25 degree C), larvae stop feeding and climb away from their food. Duration at 25 degrees C: approximately 48 hours (72-120 hours after egg laying; 48-96 hours after hatching)." [FlyBase:FBrf0007733]
comment: Temporal ordering number - 430.
synonym: "L3" EXACT []
synonym: "third instar larva" RELATED []
is_a: FBdv:00007012 ! life stage
relationship: part_of FBdv:00005336 ! larval stage
relationship: starts_at_end_of FBdv:00005338 ! second instar larval stage

[Term]
id: FBdv:00005342
name: prepupal stage
def: "The prepupal stage begins at puparium formation and ends when larval/pupal apolysis is complete, as indicated by the completion of imaginal head sac eversion and the expulsion of the oral armature of the larva. Duration at 25 degrees C: approximately 12 hours. (120-132.2 hours after egg laying; 0-12.2 hours after puparium formation)." [FlyBase:FBrf0036849, FlyBase:FBrf0048355]
comment: Temporal ordering number - 500.
is_a: FBdv:00007012 ! life stage
relationship: part_of FBdv:00007001 ! P-stage
relationship: starts_at_end_of FBdv:00005336 ! larval stage
relationship: starts_at_end_of FBdv:00005339 ! third instar larval stage

[Term]
id: FBdv:00005349
name: pupal stage
def: "The pupal stage starts once larval/pupal apolysis is complete as indicated by the expulsion of the larval armature. Early in this stage, the legs and wings reach full extension along the abdomen. The stage ends when the pupal cuticle separates from the underlying epidermis (pupal/adult apolysis), and the eye cup becomes yellow at its periphery. Duration at 25 degrees C: approximately 32 hours. (132.2-164.3 hours after egg laying; 12.2-44.3 hours after puparium formation)." [FlyBase:FBrf0036849, FlyBase:FBrf0048355]
comment: Temporal ordering number - 570. DISAMBIGUATION: In Drosophila lab vernacular, the term 'pupal stage' is often used to refer to the entire period from formation of the puparium to eclosion. However, this does not correspond to the standard usage of 'pupal stage' for Cyclorrhaphous flies (for discussion see: FBrf0087128). Briefly: formation of the puparium (hardening of the larval cuticle) marks the beginning of the pre-pupal stage. The pupal stage begins following pupal/larval apolysis - detachment of the larval epidermis from the puparium. In Drosophila, the outward sign of the completion of apolysis is the eversion of the head and expulsion of the larval mouthparts (FBrf0036849). We use P-stage to refer to the stage from pupariation to eclosion, and restrict pupal stage to its standard usage.
synonym: "phanerocephalic pupa" EXACT [FlyBase:FBrf0036849]
is_a: FBdv:00007012 ! life stage
relationship: part_of FBdv:00007001 ! P-stage
relationship: starts_at_end_of FBdv:00005342 ! prepupal stage

[Term]
id: FBdv:00005369
name: adult stage
def: "The stage of the Drosophila life-cycle from eclosion to death." [FBC:DOS]
comment: Temporal ordering number - 770.
is_a: FBdv:00007012 ! life stage
relationship: starts_at_end_of FBdv:00006011 ! pharate adult stage
relationship: starts_at_end_of FBdv:00007001 ! P-stage

[Term]
id: FBdv:00005370
name: adult stage A1
alt_id: FBdv:00005373
def: "Newly eclosed adult stage. Animal free of pupal case. Runs rapidly to find site for wing expansion. Wings are folded back and black against a very pale abdomen." [FlyBase:FBrf0049147]
comment: Temporal ordering number - 785.  The time at which eclosed flies settle down for wing expansion can vary greatly.  If they fail to find a suitable site then expansion can be delayed by several hours.
synonym: "adult stage I" RELATED []
is_a: FBdv:00005259 ! developmental stage
relationship: part_of FBdv:00007025 ! immature adult stage
relationship: starts_at_end_of FBdv:00006011 ! pharate adult stage
relationship: starts_at_end_of FBdv:00007001 ! P-stage

[Term]
id: FBdv:00005371
name: adult stage A2
alt_id: FBdv:00005374
def: "Stage, shortly after eclosion, during which the wings expand. During wing expansion, the abdomen pulsates and the hind legs stroke the wings vigorously for several minutes at a time. The stage ends when the wings are folded down over the abdomen, which has become broader and shorter, and the wing cuticle has lost its folds.  The stage lasts around 15 minutes at 25'C." [FlyBase:FBrf0049147]
comment: Temporal ordering number - 790.
synonym: "adult stage II" RELATED []
is_a: FBdv:00005259 ! developmental stage
relationship: part_of FBdv:00007025 ! immature adult stage
relationship: starts_at_end_of FBdv:00005370 ! adult stage A1

[Term]
id: FBdv:00006011
name: pharate adult stage
def: "The developing adult after pupal-adult apolysis , i.e.- from stage P8 (when yellow eye color first becomes visible through the pupal case), to eclosion. Duration at 25 degrees C: approximately 55.7 hours (164.3-220 hours after egg laying; 44.3-100 hours after puparium formation)." [FlyBase:FBrf0036849, FlyBase:FBrf0048355, FlyBase:FBrf0049147]
comment: Temporal ordering number - 625.
is_a: FBdv:00007012 ! life stage
relationship: part_of FBdv:00007001 ! P-stage
relationship: starts_at_end_of FBdv:00005349 ! pupal stage

[Term]
id: FBdv:00006012
name: adult stage A3
alt_id: FBdv:00005375
def: "Adult stage immediately after wing expansion, during which tanning of the cuticle is completed.  This stage lasts approximately 45 minutes at 25'C." [FlyBase:FBrf0049147]
comment: Temporal ordering number - 800.
synonym: "adult stage III" RELATED []
is_a: FBdv:00005259 ! developmental stage
relationship: part_of FBdv:00007025 ! immature adult stage
relationship: starts_at_end_of FBdv:00005371 ! adult stage A2

[Term]
id: FBdv:00007001
name: P-stage
def: "The stage of the Drosophila life-cycle from the formation of the puparium (beginning of the prepupal stage) to eclosion." [FBC:DOS]
comment: Temporal ordering number - 490. DISAMBIGUATION: In Drosophila lab vernacular, the term 'pupal stage' is often used to refer to the entire period from formation of the puparium to eclosion. However, this does not correspond to the standard usage of 'pupal stage' for Cyclorrhaphous flies (for discussion see: FBrf0087128). Briefly: formation of the puparium (hardening of the larval cuticle) marks the beginning of the pre-pupal stage. The pupal stage begins following pupal/larval apolysis - detachment of the larval epidermis from the puparium. In Drosophila, the outward sign of the completion of apolysis is the eversion of the head an expulsion of the larval mouthparts (FBrf0036849). We use P-stage to refer to the stage from pupariation to eclosion, and restrict pupal stage to its standard usage.
synonym: "metamorphosis" BROAD []
synonym: "pupal stage" RELATED []
is_a: FBdv:00007012 ! life stage
relationship: starts_at_end_of FBdv:00005336 ! larval stage
relationship: starts_at_end_of FBdv:00005339 ! third instar larval stage
created_by: david
creation_date: 2008-06-05T04:51:40Z

[Term]
id: FBdv:00007008
name: occurrent
equivalent_to: BFO:0000003
created_by: djs93
creation_date: 2009-10-01T05:56:28Z

[Term]
id: FBdv:00007012
name: life stage
def: "A temporal subdivision of a Drosophila life, delimited by major transitions in the circumstances of the organism, such as: fertilisation; hatching; pupal ecdysis; eclosion." [FBC:DOS]
synonym: "life cycle stage" RELATED []
is_a: FBdv:00005259 ! developmental stage
created_by: djs93
creation_date: 2009-10-01T05:59:22Z

[Term]
id: FBdv:00007025
name: immature adult stage
def: "The developmental stage that lasts from eclosion of the adult from the pupal case until tanning is complete (the end of adult stage A3)." [FBC:DOS]
comment: Temporal ordering number - 782.
is_a: FBdv:00007012 ! life stage
relationship: starts_at_end_of FBdv:00006011 ! pharate adult stage
relationship: starts_at_end_of FBdv:00007001 ! P-stage
created_by: djs93
creation_date: 2013-01-08T20:06:59Z

[Term]
id: FBdv:00007026
name: mature adult stage
def: "Life stage from the end of adult stage A3, when tanning is complete, to death." [FBC:DOS]
is_a: FBdv:00007012 ! life stage
relationship: starts_at_end_of FBdv:00006012 ! adult stage A3
relationship: starts_at_end_of FBdv:00007025 ! immature adult stage
created_by: djs93
creation_date: 2013-01-10T13:03:54Z

[Typedef]
id: ends_at_start_of
xref: RO:0002090
inverse_of: starts_at_end_of ! starts_at_end_of

[Typedef]
id: part_of
name: part_of
xref: BFO:0000050
xref: OBO_REL:part_of
is_transitive: true

[Typedef]
id: preceded_by
name: preceded_by
xref: BFO:0000062
xref: OBO_REL:preceded_by
is_transitive: true
created_by: djs93
creation_date: 2009-10-09T10:00:53Z

[Typedef]
id: starts_at_end_of
name: starts_at_end_of
xref: RO:0002087
is_a: preceded_by ! preceded_by

